Add 'valueb' Fixpoint
- This will help us make an automated 'reduce' tactic.

He4/Discussion/LanguageBase.v
@@ -60,6 +60,49 @@ Inductive value : tm -> Prop :=
   (* Classes *)
   | vcl : forall c t, value t -> value (tcl c t).
 
+Fixpoint valueb (x : tm) : bool :=
+  match x with
+  | tvoid => true
+  | tnat _ => true
+  | tbool _ => true
+  | tref _ => true
+  | trc t rc =>
+    match valueb t with
+    | true => valueb rc
+    | false => false
+    end
+  | tcl _ t => valueb t
+  | _ => false
+  end.
+
+Lemma valueb_eqiv_value:
+  forall t,
+  valueb t = true <-> value t.
+Proof with auto.
+  split.
+  - induction t; intros;
+    try solve [inversion H];
+    try solve [constructor].
+    inversion H.
+    destruct (valueb t1); destruct (valueb t2);
+    try solve [inversion H1].
+    constructor...
+    inversion H.
+    destruct (valueb t);
+    try solve [inversion H1].
+    constructor...
+  - induction t; intros; simpl;
+    try solve [inversion H];
+    try solve [reflexivity].
+    inversion H; subst.
+    apply IHt1 in H2; clear IHt1; apply IHt2 in H3; clear IHt2.
+    rewrite H2; rewrite H3.
+    reflexivity.
+    inversion H; subst.
+    apply IHt in H1; clear IHt.
+    assumption.
+  Qed.
+
 Definition stack := ProgramState.stack tm.
 Definition sk_read_hd (n : nat) (sk : stack) : tm := ProgramState.sk_read_hd n sk tvoid.
 Definition sk_resize_hd (n : nat) (sk : stack) : stack := ProgramState.sk_resize_hd n sk tvoid.
